

# Bellman Equation for $v_\pi(s)$

Alexander Schiendorfer

Pauline Steffel

July 16, 2025

Stuff we want to write  $v_\pi(s)$  in terms of:

$$\begin{aligned}\pi(a \mid s) &\stackrel{\text{def}}{=} \mathbb{P}_\pi(A_t = a \mid S_t = s) \\ p(s', r \mid s, a) &\stackrel{\text{def}}{=} \mathbb{P}(S_{t+1} = s', R_{t+1} = r \mid S_t = s, A_t = a)\end{aligned}$$

Note that  $G_t$  is the return that starts at  $R_{t+1}$ , i.e.,  $R_{t+1} + \gamma R_{t+2} + \gamma^2 R_{t+3} + \dots$ . Therefore  $G_{t+1} = R_{t+2} + \gamma R_{t+3} + \dots$ . Some useful sets:

- $a \in A$ :  $a$  is a specific action (e.g., “left” or “right”);  $A$  is the set of all actions
- $r \in R \subseteq \mathbb{R}$ :  $r$  is a specific reward,  $R$  is the set of all possible rewards, e.g.  $R = \{-15, -5, 0, 5, 15\}$
- $s' \in S$ :  $s'$  is a specific next state,  $S$  is the set of all states

Expected value of a random variable  $X$ :

$$\mathbb{E}[X] = \sum_x x \cdot \mathbb{P}(X = x) \quad (1)$$

Conditional expectation of a random variable  $X$  given another random variable  $Y$ :

$$\mathbb{E}[X \mid Y = y] = \sum_x x \cdot \mathbb{P}(X = x \mid Y = y) \quad (2)$$

Partition theorem or law of total expectation:

$$\mathbb{E}[X] = \sum_y \mathbb{P}(Y = y) \mathbb{E}[X \mid Y = y] \quad (3)$$

Linearity of expectation:

$$\mathbb{E}[X + Y] = \mathbb{E}[X] + \mathbb{E}[Y] \quad (4)$$

Marginal probabilities of joint probabilities:

$$\mathbb{P}(X = x) = \sum_y \mathbb{P}(X = x, Y = y) \quad (5)$$

Definition of  $v_\pi(s)$ :

$$v_\pi(s) \stackrel{\text{def}}{=} \mathbb{E}_\pi[G_t \mid S_t = s]$$

Pull one reward out of the return (the return is just a random variable that sums rewards with discounting):

$$v_\pi(s) = \mathbb{E}_\pi[R_{t+1} + \gamma G_{t+1} \mid S_t = s]$$

Apply Equation (3) to condition the expectation on actions; “pull out” the action  $A_t$  as the random variable  $Y$  in Equation (3):

$$v_\pi(s) = \sum_a \underbrace{\mathbb{P}_\pi(A_t = a \mid S_t = s)}_{\pi(a \mid s)} \mathbb{E}_\pi[R_{t+1} + \gamma G_{t+1} \mid S_t = s, A_t = a]$$

Split the expectation of a sum into a sum of expectations by using the linearity of expectation from Equation (4) (note that given an action, the expected immediate reward doesn’t depend on the policy):

$$v_\pi(s) = \sum_a \mathbb{P}_\pi(A_t = a \mid S_t = s) (\mathbb{E}[R_{t+1} \mid S_t = s, A_t = a] + \mathbb{E}_\pi[\gamma G_{t+1} \mid S_t = s, A_t = a])$$

Pull out  $\gamma$  by linearity of expectation:

$$v_\pi(s) = \sum_a P_\pi(A_t = a \mid S_t = s) (\mathbb{E}[R_{t+1} \mid S_t = s, A_t = a] + \gamma \mathbb{E}_\pi[G_{t+1} \mid S_t = s, A_t = a])$$

Write just the expected **immediate** reward  $R_{t+1}$  in terms of  $p(s', r \mid s, a)$ :<sup>1</sup>

$$v_\pi(s) = \sum_a P_\pi(A_t = a \mid S_t = s) \left( \sum_{s', r} r \cdot P(S_{t+1} = s', R_{t+1} = r \mid S_t = s, A_t = a) + \gamma \mathbb{E}_\pi[G_{t+1} \mid S_t = s, A_t = a] \right)$$

Now we apply Equation (3) to condition the other expectation on the next state  $S_{t+1}$ , basically we “pull out” the next state  $S_{t+1}$  as the random variable  $Y$  in Equation (3):

$$v_\pi(s) = \sum_a P_\pi(A_t = a \mid S_t = s) \left( \sum_{s', r} r \cdot P(S_{t+1} = s', R_{t+1} = r \mid S_t = s, A_t = a) + \gamma \sum_{s'} P(S_{t+1} = s' \mid S_t = s, A_t = a) \mathbb{E}_\pi[G_{t+1} \mid S_t = s, A_t = a, S_{t+1} = s'] \right)$$

By the Markov property, knowing  $S_{t+1}$  makes the expectation independent of  $S_t$  and  $A_t$ :

$$v_\pi(s) = \sum_a P_\pi(A_t = a \mid S_t = s) \left( \sum_{s', r} r \cdot P(S_{t+1} = s', R_{t+1} = r \mid S_t = s, A_t = a) + \gamma \sum_{s'} P(S_{t+1} = s' \mid S_t = s, A_t = a) \mathbb{E}_\pi[G_{t+1} \mid S_{t+1} = s'] \right)$$

By stationarity of the MDP, we know that starting in some state  $s'$  will bring the same expected return, regardless of whether this is at time step  $t$  or  $t+1$ ,  $\mathbb{E}_\pi[G_{t+1} \mid S_{t+1} = s'] = \mathbb{E}_\pi[G_t \mid S_t = s']$  and thus  $v_\pi(s')$ :

Acknowledging that  $v_\pi(s') = \mathbb{E}_\pi[G_{t+1} \mid S_{t+1} = s']$ , and combining the summations:

$$v_\pi(s) = \sum_a P_\pi(A_t = a \mid S_t = s) \left( \sum_{s', r} r \cdot P(S_{t+1} = s', R_{t+1} = r \mid S_t = s, A_t = a) + \gamma \sum_{s'} P(S_{t+1} = s' \mid S_t = s, A_t = a) v_\pi(s') \right)$$

To get both summations into one, we can just write the joint probability of  $S_{t+1}$  and  $R_{t+1}$  and “demarginalize” according to eq. (5) applied backwards:

$$v_\pi(s) = \sum_a P_\pi(A_t = a \mid S_t = s) \left( \sum_{s', r} r \cdot P(S_{t+1} = s', R_{t+1} = r \mid S_t = s, A_t = a) + \gamma \sum_{s', r} P(S_{t+1} = s', R_{t+1} = r \mid S_t = s, A_t = a) v_\pi(s') \right)$$

which we can now combine into one summation:

$$v_\pi(s) = \sum_a P_\pi(A_t = a \mid S_t = s) \left( \sum_{s', r} r \cdot P(S_{t+1} = s', R_{t+1} = r \mid S_t = s, A_t = a) + \gamma P(S_{t+1} = s', R_{t+1} = r \mid S_t = s, A_t = a) v_\pi(s') \right)$$

now pulling out  $P(S_{t+1} = s', R_{t+1} = r \mid S_t = s, A_t = a)$ :

---

<sup>1</sup>Honestly, we wouldn't have to average this over all subsequent states here, we could have marginalized (see eq. (5)) over the next state  $S_{t+1}$ , to get just the probabilities over  $R_{t+1}$ :  $v_\pi(s) = \sum_a P_\pi(A_t = a \mid S_t = s) (\sum_r r \cdot P(R_{t+1} = r \mid S_t = s, A_t = a) + \gamma \mathbb{E}_\pi[G_{t+1} \mid S_t = s, A_t = a])$  but we did it to make the next steps easier.

$$v_{\pi}(s) = \sum_a P_{\pi}(A_t = a \mid S_t = s) \left( \sum_{s', r} P(S_{t+1} = s', R_{t+1} = r \mid S_t = s, A_t = a) \cdot (r + \gamma v_{\pi}(s')) \right)$$

and that, in fact, can just be written as an expected value using the definition of the expected value (Equation (1)), in particular conditioned on the the current state  $S_t = s$  and action  $A_t = a$  (Equation (2)):

$$v_{\pi}(s) = \sum_a P_{\pi}(A_t = a \mid S_t = s) \left( \mathbb{E}_{S_{t+1}, R_{t+1}} [R_{t+1} + \gamma v_{\pi}(S_{t+1}) \mid S_t = s, A_t = a] \right)$$

and, finally, using the law of total expectation (Equation (3)) over the action  $A_t$  as the random variable  $Y$  in Equation (3):

$$v_{\pi}(s) = \mathbb{E}_{\pi}(R_{t+1} + \gamma v_{\pi}(S_{t+1}) \mid S_t = s)$$